\input{../../templateExo.tex}

\begin{document}
\hrulefill

\begin{minipage}{0.33\textwidth}
\textsc{Math 471}
\end{minipage} \hfill 
\begin{minipage}{0.32\textwidth}
\centering
\textsc{Solutions to Problems} \\
Chapter F
\end{minipage}
 \hfill 
 \begin{minipage}{0.33\textwidth}
 \flushright \textsc{Fall 2023}
 \end{minipage}

\hrulefill

\setcounter{section}{6}

\subsection{Moments}

\begin{problem}
From the definition of the $k$-th moment, we compute
    \[
        \mathrm{Exp} (X^k) = \int_{-\infty}^\infty x^k f_X (x) \, dx = \int_a^b \frac{x^k}{b - a} \, dx .
    \]
After integrating $x^k$, we obtain the answer:
    \[
        \mathrm{Exp} (X^k) = \frac{b^{k + 1} - a^{k + 1}}{(k + 1) (b - a)} . \tag*{$\triangle$}
    \]
\end{problem}

\subsection{Moment Generating Function}

\begin{problem}
The moment generating function of the normal distribution is
    \[
        M_X (t) = e^{\mu_X t + \frac{1}{2}\sigma_X^2 t^2} .
    \]
Since $\mu_X = 0$ and $\sigma_X^2 = 1$, we then get $M_X (t) = e^{t^2/2}$. From Theorem F.1, we know that
    \[
        \mathrm{Exp} (X^3 ) = M_X^{(3)} (0) .
    \]
We have
    \[
        M_X^{(3)} (t) = e^{t^2/2} t (t^2 + 3) \quad \Rightarrow \quad \mathrm{Exp} (X^3) = 0 .\tag*{$\triangle$}
    \]
\end{problem}

\begin{problem}
We will identify the moment generating function of $aX + b$. From the definition of the moment generating function, we have
    \[  
        M_{aX + b} (t) = \mathrm{Exp} (e^{t(aX + b)}) = e^{tb} \mathrm{Exp} (e^{taX}) = e^{tb} M_X (at ) .
    \]
Since $X \sim N (\mu_X , \sigma_X )$, we know that $M_X (t) = e^{\mu_X t + \frac{1}{2} \sigma_X^2 t^2}$. Substituting this into the equation for $M_{aX + b} (t)$, we find that
    \[
        M_{aX + b} (t) = e^{tb} e^{\mu_X at + \frac{1}{2} \sigma_X^2 a^2 t^2} = e^{(b + \mu_X a) t + \frac{1}{2} \sigma_X^2 a^2 t^2} .
    \]
The moment generating function of $aX + b$ is then the moment generating function of a normal distribution with average $b + \mu_X a$ and variance $\sigma_X^2 a^2$. Hence, $aX + b \sim N (b + \mu_X a , \sigma_X^2 a^2 )$. \hfill $\triangle$
\end{problem}

\begin{problem}
    \begin{enumerate}[label=\alph*)]
        \item Since $X$ is an exponential distribution and $\lambda = 1/\theta$, we find that
            \[
                M_X (t) = \frac{1/\theta}{1/\theta - t} = \frac{1}{1 - \theta t} , 
            \]
        for $t < 1/\theta$.
        \item We know that
            \[
                \mathrm{Exp} (X) = M'_X (0) \quad \text{ and } \quad \mathrm{Var} (X) = \mathrm{Exp} (X^2) - (\mathrm{Exp} (X))^2 = M''_X (0) - (M'_X(0))^2 .
            \]
        We compute
            \[
                M_X' (t) = \frac{\theta}{(1 - \theta t)^2} \quad \text{ and } \quad M_X'' (t) = \frac{2\theta^2}{(1 - \theta t)^{3}}
            \]
        Hence
            \[
                \mathrm{Exp} (X) = \frac{\theta}{(1 - \theta (0))^2} = \theta
            \]
        and
            \[
                \mathrm{Var} (X) = \frac{2\theta^2}{(1 - \theta (0))^3} - (\theta)^2 = \theta^2 . \tag*{$\triangle$}
            \]
    \end{enumerate}
\end{problem}

\end{document}